theories/program_logic/idiverges.v
@@ -1,0 +1,172 @@
+From Paco Require Import
+  paco.
+
+From iris.bi Require Import
+  fixpoint.
+From iris.base_logic Require Import
+  lib.iprop.
+From iris.proofmode Require Import
+  proofmode.
+
+From simuliris Require Import
+  prelude.
+From simuliris.common Require Import
+  tactics.
+From simuliris.base_logic Require Import
+  satisfiable.
+From simuliris.program_logic Require Import
+  language.
+
+Section bi.
+  Context `{!BiBUpd PROP} `{!BiAffine PROP}.
+  Context {Λ : language}.
+  Context (prog : program Λ).
+  Implicit Types N I : expr_O Λ -d> state_O Λ -d> PROP.
+
+  Definition idiverges_body N : expr_O Λ -d> state_O Λ -d> PROP := (
+    λ e σ,
+      ∃ e' σ', ⌜prim_step prog e σ e' σ'⌝ ∗ N e' σ'
+  )%I.
+
+  #[local] Definition idiverges_body' (N : prodO (expr_O Λ) (state_O Λ) -d> PROP) : prodO (expr_O Λ) (state_O Λ) → PROP :=
+    uncurry $ idiverges_body $ curry N.
+  #[local] Definition idiverges_def : expr_O Λ -d> state_O Λ -d> PROP :=
+    curry $ bi_greatest_fixpoint idiverges_body'.
+  #[local] Definition idiverges_aux :
+    seal (@idiverges_def). Proof. by eexists. Qed.
+  Definition idiverges :=
+    idiverges_aux.(unseal).
+  #[local] Definition idiverges_unseal : @idiverges = @idiverges_def :=
+    idiverges_aux.(seal_eq).
+
+  #[global] Instance idiverges_body_ne n :
+    Proper ((≡{n}≡) ==> (=) ==> (=) ==> (≡{n}≡)) idiverges_body.
+  Proof.
+    solve_proper.
+  Qed.
+  #[global] Instance idiverges_body_proper :
+    Proper ((≡) ==> (=) ==> (=) ==> (≡)) idiverges_body.
+  Proof.
+    solve_proper.
+  Qed.
+
+  Lemma idiverges_body_mono N1 N2 e σ :
+    (∀ e' σ', N1 e' σ' -∗ N2 e' σ') -∗
+    idiverges_body N1 e σ -∗
+    idiverges_body N2 e σ.
+  Proof.
+    iIntros "HN (%e' & %σ' & %Hstep & HN1)".
+    iExists e', σ'. iSplit; first done. iApply ("HN" with "HN1").
+  Qed.
+
+  #[local] Instance idiverges_body'_ne n :
+    Proper ((≡{n}≡) ==> (=) ==> (≡{n}≡)) idiverges_body'.
+  Proof.
+    intros N1 N2 HN (e1, σ1) (e2, σ2) <-.
+    rewrite /idiverges_body' /=. f_equiv. intros e σ. apply HN.
+  Qed.
+  #[local] Instance idiverges_body'_proper :
+    Proper ((≡) ==> (=) ==> (≡)) idiverges_body'.
+  Proof.
+    intros N1 N2 HN (e1, σ1) (e2, σ2) <-.
+    rewrite /idiverges_body' /=. f_equiv. intros e σ. apply HN.
+  Qed.
+  #[local] Instance idiverges_body'_mono_pred :
+    BiMonoPred idiverges_body'.
+  Proof.
+    split; last solve_proper.
+    iIntros "%N1 %N2 %HN1 %HN2 #HN" ((e, σ)) "/=".
+    iApply idiverges_body_mono. iIntros "%e' %σ' HN1".
+    iApply ("HN" with "HN1").
+  Qed.
+
+  Lemma idiverges_fixpoint e σ :
+    idiverges e σ ⊣⊢
+    idiverges_body idiverges e σ.
+  Proof.
+    rewrite idiverges_unseal.
+    setoid_rewrite greatest_fixpoint_unfold; [done | apply _].
+  Qed.
+  Lemma idiverges_unfold e σ :
+    idiverges e σ -∗
+    idiverges_body idiverges e σ.
+  Proof.
+    rewrite idiverges_fixpoint //.
+  Qed.
+  Lemma idiverges_fold e σ :
+    idiverges_body idiverges e σ -∗
+    idiverges e σ.
+  Proof.
+    rewrite idiverges_fixpoint //.
+  Qed.
+
+  Lemma idiverges_strong_coind I e σ :
+    □ (
+      ∀ e σ,
+      I e σ -∗
+        ∃ e' σ',
+        ⌜tc (step prog) (e, σ) (e', σ')⌝ ∗
+        (I e' σ' ∨ idiverges e σ)
+    ) -∗
+    I e σ -∗
+    idiverges e σ.
+  Proof.
+    assert (BiMonoPred (λ (N : _ → _) x, uncurry I x ∨ idiverges_body' N x)%I) as Hmono.
+    { clear dependent e σ. split.
+      - iIntros "%N1 %N2 %HN1 %HN2 #HN" ((e, σ)) "[HI | HN1]"; first auto.
+        iRight. iApply (idiverges_body_mono with "[] HN1"). iIntros "%e' %σ'".
+        iApply "HN".
+      - intros N HN n (e1, σ1) (e2, σ2) (He%leibniz_equiv & Hσ%leibniz_equiv).
+        solve_proper.
+    }
+    rewrite idiverges_unseal.
+    iIntros "#Hind HI".
+    replace (I e σ) with ((uncurry I) (e, σ)); last done.
+    iApply (greatest_fixpoint_paco with "[] HI"). clear e σ. iIntros "!>" ((e, σ)) "HI /=".
+    iDestruct ("Hind" with "HI") as "(%e'' & %σ'' & %Hsteps & [HI | Hidiv])"; iClear "Hind"; last first.
+    { rewrite -idiverges_unseal idiverges_fixpoint.
+      iApply (idiverges_body_mono with "[] Hidiv"). iIntros "%e' %σ' Hidiv".
+      rewrite idiverges_unseal /idiverges_def /curry /Datatypes.curry /=.
+      iApply (greatest_fixpoint_strong_mono with "[] Hidiv"). clear dependent e σ. iIntros "!> %N" ((e, σ)) "Hidiv".
+      auto.
+    }
+    match goal with |- _ _ ?P =>
+      enough (I e'' σ'' -∗ P) as H; first iApply (H with "HI")
+    end.
+    remember (e, σ) as cfg. remember (e'', σ'') as cfg''.
+    revert dependent σ. revert dependent e.
+    induction Hsteps as [? ? Hstep | ? (e', σ') ? Hstep Hsteps IH]; iIntros (e σ ->) "HI"; simplify.
+    - iExists e'', σ''. iSplit; first auto using step_prim_step.
+      setoid_rewrite greatest_fixpoint_unfold; auto.
+    - iExists e', σ'. iSplit; first auto using step_prim_step.
+      setoid_rewrite greatest_fixpoint_unfold; last done.
+      iRight. iApply (IH with "HI"); done.
+  Qed.
+  Lemma idiverges_coind I e σ :
+    □ (
+      ∀ e σ,
+      I e σ -∗
+        ∃ e' σ',
+        ⌜tc (step prog) (e, σ) (e', σ')⌝ ∗
+        I e' σ'
+    ) -∗
+    I e σ -∗
+    idiverges e σ.
+  Proof.
+    iIntros "#Hind HI".
+    iApply (idiverges_strong_coind with "[] HI"). clear e σ. iIntros "!> %e %σ HI".
+    iDestruct ("Hind" with "HI") as "(%e' & %σ' & %Hsteps & HI)".
+    auto.
+  Qed.
+End bi.
+
+Lemma idiverges_adequacy Σ Λ (prog : program Λ) e σ :
+  (⊢@{iPropI Σ} idiverges prog e σ) →
+  diverges prog e σ.
+Proof.
+  intros Hidiv%isat_intro.
+  revert dependent σ. revert dependent e. pcofix CIH. intros e σ.
+  rewrite idiverges_fixpoint.
+  intros (e' & (σ' & (Hstep%satisfiable_elim & Hisat)%satisfiable_sep)%satisfiable_exists)%satisfiable_exists.
+  pfold. econstructor; first done. right. apply CIH. done.
+Qed.
